# The Operator Formalism







## Descendant States and Fields

### Descendants States

#### Conformal Operators Acting on the Vacuum State

The energy of the ground state is fixed to zero. This requires that

$$
T(z)|0\rangle
= \sum_n z^{-n-2} L_n |0\rangle
$$

and the anti-holomorphic $\bar{T}(\bar{z}) |0\rangle$ are well-defined as $z, \bar{z} \to 0$ (no divergence). Then we must have

$$
\begin{cases}
    L_n|0\rangle =0 \\
    \bar{L}_n|0\rangle =0
\end{cases}
\quad
\text{for } -n - 2 \le -1 
\text{ or } n \ge -1
$$

These include the invariance of the vacuum with respect to the *global* conformal transformations generated by $L_{-1},L_0,L_1$ and their anti-holomorphic counterparts, which means that $|0\rangle$ *must be annihilated by these operators*.

Now we also have

$$
\langle 0| T(z) |0\rangle 
= \langle 0 | \bar{T}(\bar{z}) | 0\rangle =0
$$

#### Conformal Operators Acting on the Asymptotic State

Consider the $L_n, \bar{L}_n$ operators acting on the *asymptotic state*

$$
|h,\bar{h} \rangle 
\equiv \phi(0,0) |0\rangle
$$

Here $\phi(z, \bar{z})$ is a *primary field* with conformal dimensions $(h, \bar{h})$. Because we have already know the action on the vacuum, we may calculate

$$
[L_n,\phi(0,0)] |0\rangle 
= L_n\phi(0,0)|0\rangle -  \phi(0,0)L_n|0\rangle
$$

When $n\ge -1$, the second term vanishes. Then

$$
[L_n,\phi(0,0)] |0\rangle 
= L_n\phi(0,0) |0\rangle 
= L_n |h,\bar{h} \rangle
$$

Now we evaluate the commutator

$$
\begin{aligned}
    [L_n,\phi(w,\bar{w})]
    &= \frac{1}{2 \pi i} \oint_w dz \,
    z^{n+1} \underbrace{T(z)\phi(w,\bar{w})}_{\text{use OPE}} 
    \\
    &= \frac{1}{2 \pi i} \oint_w dz \,
    z^{n+1} \left[
        \frac{h \phi(w,\bar{w})}{(z-w)^2}
        + \frac{\partial_w\phi(w,\bar{w})}{z-w}
        + \text{reg.}
    \right]
    \\
    &= \left[
        \frac{d}{dz} \left(z^{n+1}h \phi(w,\bar{w})\right)
    \right]_{z=w} + \left[
        z^{n+1} \partial_w\phi(w,\bar{w})
    \right]_{z=w} 
    \\
    &= h(n+1) w^n \phi(w,\bar{w})
    + w^{n+1} \partial_w \phi(w,\bar{w})
\end{aligned}
$$

Similarly

$$
[\bar{L}_n, \phi(w,\bar{w})]
= \bar{h}(n+1)\bar{w}^n \phi(w,\bar{w})
+ \bar{w}^{n+1} \partial_{\bar{w}} \phi(w,\bar{w})
$$

Finally

$$
\begin{aligned}
    L_0|h,\bar{h} \rangle &= h|h,\bar{h} \rangle
    \\
    \bar{L}_0|h,\bar{h} \rangle &= \bar{h}|h,\bar{h} \rangle
    \\ 
    L_n|h,\bar{h} \rangle &= 0
    \\
    \bar{L}_n|h,\bar{h} \rangle &= 0
    \qquad (n > 0)
\end{aligned}
$$

Since $L_0+\bar{L}_0$ is proportional to the system Hamiltonian, we find
that $|h,\bar{h} \rangle$ *is an energy eigenstate*.

### Ladder Operators

To find excited states above the asymptotic state, we need the *ladder operators*. It turns out that they can be chosen as the *Laurent modes* $\phi_n$ *of the holomorphic field* $\phi(w)$ *with conformal dimension* $h$.

$$
\phi(z) = \sum_n z^{-n-h} \phi_n, \quad
\phi_n = \frac{1}{2 \pi i} \oint dz \, z^{n+h-1} \phi(z)
$$

To show this, we calculate the commutator $[L_n, \phi_m]$ using the equation

$$
[A,B] = \oint_0 dw \oint_w dz \, a(z) b(w)
$$

Recall that

$$
L_n = \frac{1}{2 \pi i} \oint dz z^{n+1} T(z)
$$

then

$$
\begin{aligned}
    &\left[L_n,\phi_m\right]
    \\
    &= \frac{1}{2 \pi i} \oint_0 dw \, w^{m+h-1} 
    \frac{1}{2 \pi i} \oint_w dz \, z^{n+1}T(z)\phi(w)
    \\
    &= \frac{1}{2 \pi i} \oint_0 dw \, w^{m+h-1} 
    \frac{1}{2 \pi i} \oint_w dz \, z^{n+1} 
    \left[
        \frac{h \phi(w)}{(z-w)^2}
        + \frac{\partial_w\phi(w)}{z-w}
        + \text{reg.}
    \right]
    \\
    &= \frac{1}{2 \pi i} \oint_0 dw w^{m+h-1} 
    \left(
        h (n+1) w^n \phi(w) 
        + w^{n+1} \partial_w \phi(w)
    \right)
    \\
    &= \frac{1}{2 \pi i} \oint_0 dw \left(
        h (n+1) w^{m+n+h-1} \phi(w)
        + \underbrace{w^{m+n+h} \partial_w\phi(w)}_{\text{integrate by parts}}
    \right)
    \\
    &= \frac{1}{2 \pi i} \oint_0 dw \left(
        h(n+1)w^{m+n+h-1} \phi(w)
        - (m+n+h) w^{m+n+h-1} \phi(w)
    \right)
    \\
    &= \frac{1}{2 \pi i} \oint_0 dw 
    (n(h-1)-m) w^{m+n+h-1} \phi(w)
\end{aligned}
$$

This implies that

$$
[L_n, \phi_m] = (n(h-1)-m) \phi_{n+m}
$$

In particular,

$$
\begin{aligned}
    [L_0, \phi_m] &= -m \phi_m\\
    [L_0, \phi_{-m}] &= m \phi_{-m}
\end{aligned}
$$

This means that $\phi_{\pm m} (m>0)$ act as *lowering and raising operators for the eigenstates of* $L_0$: from $L_0|h\rangle =h|h\rangle$ we obtain

$$
\begin{aligned}
    L_0 (\phi_{\pm m}|h\rangle )
    &= [L_0, \phi_{\pm m}] |h\rangle 
    + \phi_{\pm m} L_0 |h\rangle 
    \\
    &= \mp m \phi_{\pm m} |h\rangle 
    + h \phi_{\pm m} |h\rangle 
    \\
    &= (h\mp m) (\phi_m |h\rangle)
\end{aligned}
$$

i.e. $\phi_{\pm m}|h\rangle$ is the eigenstate of $L_0$ with
eigenvalue $h\mp m$.

But we still have another choice. Recall that in the Virasoro algebra

$$
[L_n, L_m] 
= (n-m) L_{n+m}
+ \frac{c}{12} n (n^2 - 1) \delta_{n+m, 0}
$$

Specially, for $n=0$

$$
\begin{aligned}
    [L_0, L_m] &= -m L_m\\
    [L_0, L_{-m}] &= m L_{-m}
\end{aligned}
$$

which has the *same* form as $\left[L_0,\phi_{\pm m} \right]$. Therefore, $L_{\pm m} (m>0)$ can also *lower and raise the conformal dimension*.

Finally, we remark that

$$ L_{-n}=L_n^\dagger $$

### Descendant States

The state

$$
L_{-k_1}L_{-k_2} \cdots L_{-k_n}|h\rangle 
\qquad (1 \le k_1 \le \cdots \le k_n)
$$

is an eigenstate of $L_0$ with eigenvalue

$$
h' = h + N, \quad 
N \equiv k_1 + k_2 + \cdots + k_n
$$

We call such kind of states **descendant states** (or simply **descendants**) of the asymptotic state $|h\rangle$, although this name is a little bit weird considering that they are produced by *raising* operators $L_{-n}$. The integer $N$ is called the **level** of the descendant.

*Theorem*: Descendant states belonging to different levels are orthogonal.

*Proof*:

- We first consider the simple case

    $$
    |i\rangle =L_{-M}|h\rangle , \quad |j\rangle =L_{-N}|h\rangle
    \quad (N, M > 0, N \ne M)
    $$

    In the following calculation, since $L_n$ are not Hermitian, we can only apply them to *kets*. Then

    $$
    \begin{aligned}
        \langle i|j \rangle 
        &= \langle h | L_M L_{-N} | h \rangle 
        = \langle h | L_{-N} L_M + [L_M,L_{-N}] | h \rangle
        \\
        &=\langle h|L_{-N} \underbrace{L_M|h\rangle}_0
        \\ &\qquad
        + \left\langle h \left|
            (M-N) L_{M-N} 
            + \frac{c}{12} M (M^2-1) \delta_{M+N, 0} 
        \right| h\right\rangle
        \\
        &=(M-N)\left\langle h\left|L_{M-N} \right|h\right\rangle
    \end{aligned}
    $$

    Without loss of generality, assume $M>N$, then $L_{M-N}|h\rangle =0$, and we proved that $\langle i|j\rangle =0$. 
    
    (If $M<N$, we can calculate its the complex conjugate $\left\langle h\left|L_{N-M} \right|h\right\rangle =0$, so it is also zero)

- In general, let

    $$
    \begin{aligned}
        |i\rangle &= L_{-k_1} \cdots L_{-k_m}|h\rangle , 
        &\quad 
        &k_1 + \cdots + k_m = M
        \\
        |j\rangle &= L_{-l_1} \cdots L_{-l_n}|h\rangle , 
        &\quad
        &l_1 + \cdots + l_n = N \ne M
    \end{aligned}
    $$

    We calculate

    $$
    \langle i|j\rangle 
    = \langle h | 
        L_{k_m} \cdots L_{k_1}
        L_{-l_1} \cdots L_{-l_n}
    | h \rangle
    $$




### Descendant Fields

Each descendant state can be regarded as the result of the application on the vacuum of a **descendant field**. 

For example, consider the simplest level-$n$ descendant state, for which the integer $n$ is not partitioned at all

$$
L_{-n}|h\rangle =L_{-n} \phi(0)|0\rangle
$$

The descendant field $\phi^{(-n)}$ associated with this state should
satisfy

$$
\phi^{(-n)}(0)|0\rangle =L_{-n}|h\rangle
$$

Since $L_{-n}$ is a Laurent mode of $T(z)$, we can write

$$
L_{-n}|h\rangle =\frac{1}{2 \pi i} \oint dz z^{-n+1}T(z)\phi(0)|0\rangle
$$

Then the descendant field $\phi^{(-n)}$ can be naturally chosen as

$$
\begin{aligned}
    \phi^{(-n)}(w)
    &= \frac{1}{2 \pi i} \oint_w dz (z-w)^{-n+1}T(z)\phi(w)
    \\
    &= L_{-n}(w)\phi(w)
    \\
    &\equiv \left(L_{-n} \phi \right)(w)
\end{aligned}
$$

As two special cases, according to the general formulas

$$
\left(L_0 A\right)(w) = h_A A(w), \quad
\left(L_{-1} A\right)(w) = \partial_w A(w)
$$

we find

$$
\phi^{(0)}(w) = h \phi(w), \quad
\phi^{(-1)}(w) = \partial \phi(w)
$$

In general, we can partition $n$ into $m$ numbers $k_1+k_2+\cdots+k_m$ and define recursively the corresponding
descendant field as

$$
\begin{aligned}
    &\phi^{\left(-k_1,-k_2,\cdots,k_m\right)}(w)
    = (L_{-k_1}L_{-k_2} \cdots L_{-k_m} \phi)(w)
    \\
    &= \frac{1}{2 \pi i} \oint_w dz \, 
    (z-w)^{-k_1+1} T(z) \phi^{(-k_2,...,-k_m)}(w)
\end{aligned}
$$

In particular, we need to emphasize that $\phi^{(0,-n)}$ is *not* the same as $\phi^{(-n)}$:

$$
\phi^{(0,-n)}(w) = (h+n)\phi^{(-n)}(w)
$$

Another commonly used relation is

$$ 
\phi^{(-1,-n)}(w) = \partial \phi^{(-n)}(w)
$$

### A Representation of the Conformal Generators

The relations $\phi^{(-1)}(w)=\partial \phi(w)$ and
$\phi^{(-1,-n)}(w)=\partial \phi^{(-n)}(w)$ give us the first hint that $L_{-1}(w)$ somewhat has the same effect as the differential operator $\partial_w$. 

To illustrate what this exactly means, let $X\equiv \phi_1(w_1) \cdots \phi_N(w_N)$ and consider the correlation function

$$
\langle \phi^{(-n)}(w)X \rangle 
\equiv \langle (L_{-n} \phi)(w) X \rangle
$$

we can find a differential operator $\mathcal{L}_{-n}$ such that

$$
\left\langle \left(L_{-n} \phi \right)(w)X\right\rangle =\mathcal{L}_{-n} \langle \phi(w)X\rangle \text{   }(n\ge 1)
$$

with

$$
\mathcal{L}_{-n}
= \sum_{i=1}^N \left[
    \frac{(n-1)h_i}{\left(w_i-w\right)^n}
    - \frac{1}{\left(w_i-w\right)^{n-1}} \partial_{w_i} 
\right]
$$

In particular

$$
\mathcal{L}_{-1} = \partial_w
$$

*Proof*:

*Remarks*:

1. In general

    $$
    \langle \phi^{(-k_1, ..., -k_m)}(w)\, X \rangle 
    =\mathcal{L}_{-k_1} \cdots \mathcal{L}_{-k_m} 
    \langle \phi(w)X\rangle
    $$

2. Recall the most primitive operators in Witt algebra

    $$
    l_{-n}=-w^{-n+1} \partial_w
    $$

### Conformal Families

The set consisting of a *primary field* $\phi$ and *all of its descendants* is called a **conformal family**, sometimes denoted by $[\phi]$. The members of a family *transform amongst themselves under conformal transformations*.

### OPE of $T(z)$ with Descendant Fields

### The Operator Algebra

### Conformal Blocks

