## Energy-Momentum Tensor in 2D 

----

*Proposition*: Energy-Momentum Tensor in CFT is Traceless

*Proof*: From general quantum field theory, when we perform an infinitesimal spacetime translation

$$
x'^\mu = x^\mu + \epsilon^\mu(x)
$$

the variation of action is given by

$$
\delta S = \int d^d x \, 
\epsilon^\nu \partial_\mu {T^\mu}_{\nu}
$$

from which we require, if the system is symmetric under the translation

$$
\partial_\mu T^{\mu \nu} = 0
$$

Now we let $\epsilon^\mu(x)$ be generated by an infinitesimal conformal transformation. 

----

In the following we consider E-M tensors in 2D. 

### Holomorphic Components of the Energy-Momentum Tensor 

The energy-momentum tensor $T_{\mu  \nu}$ transforms in the same way as the metric $g_{\mu  \nu}$:

$$
\begin{aligned}
    T'_{\mu \nu}
    &= \begin{pmatrix}
        T_{zz} & T_{z \bar{z}} \\
        T_{\bar{z} z} & T_{\bar{z}\bar{z}}
    \end{pmatrix}
    = T_{\rho \sigma}
    \frac{\partial x^\rho}{\partial z^\mu}
    \frac{\partial x^\sigma}{\partial z^\nu}
\end{aligned}
$$

For example:

$$
\begin{aligned}
    T_{z z} 
    &=
    \frac{\partial x^0}{\partial z} \frac{\partial x^0}{\partial z}T_{00}
    + \frac{\partial x^0}{\partial z} \frac{\partial x^1}{\partial z}T_{01}
    \\ &\qquad
    +\frac{\partial x^1}{\partial z} \frac{\partial x^0}{\partial z}T_{10}
    + \frac{\partial x^1}{\partial z} \frac{\partial x^1}{\partial z}T_{11}
    \\
    &= \frac{1}{2} \frac{1}{2}T_{00}
    + \frac{1}{2} \frac{-i}{2}T_{01}
    + \frac{-i}{2} \frac{1}{2}T_{10}
    + \frac{-i}{2} \frac{-i}{2}T_{11}
    \\
    &= \frac{1}{4} (T_{00} - 2i T_{10} - T_{11})
\end{aligned}
$$

Proceeding in the same way, we find

$$
\begin{aligned}
    T_{\bar{z} \bar{z}} 
    &= \frac{1}{4} (T_{00} + 2i \, T_{10} - T_{11})
    \\
    T_{z \bar{z}} = T_{\bar{z}z}
    &= \frac{1}{4} (T_{00}+T_{11})
\end{aligned}
$$

Since the energy-momentum tensor for 2D CFT is *traceless*, we can further simplify the relations to:

$$
\begin{aligned}
    T_{z z}
    &= \frac{1}{2} (T_{00}-i T_{10})
    \\
    T_{\bar{z} \bar{z}}
    &=\frac{1}{2} (T_{00}+i T_{10})
    \\
    T_{z \bar{z}} = T_{\bar{z}z} &=0
\end{aligned}
$$

We now show that $T_{z z},T_{\bar{z} \bar{z}}$ depends only on $z$ and $\bar{z}$ respectively, so we define

$$
T(z)\equiv -2\pi  T_{z z}(z), 
\quad
\bar{T}(\bar{z}) \equiv -2\pi T_{\bar{z} \bar{z}}(\bar{z})
$$

*Proof*:

Recall that

$$
\partial^{\mu}T_{\mu  \nu}=0
$$

In *Euclidean* spacetime, this is explicitly

$$
\partial_0T_{00}+\partial_1T_{10}
= \partial_0T_{01}+\partial_1T_{11}
= 0
$$

Since the energy-momentum tensor is traceless and symmetric:

$$
\begin{aligned}
    \partial_{\bar{z}}T_{z z}
    &= \frac{1}{4} 
    (\partial_0 + i\partial_1)
    (T_{00} - i T_{10})
    \\
    &= \frac{1}{4} (
        \partial_0T_{00}
        - i \partial_0 T_{10}
        + i \partial_1 T_{00}
        +\partial_1T_{10}
    )
    \\
    &= \frac{1}{4} (
        \partial_0T_{00}
        - i \partial_0 T_{01}
        - i \partial_1 T_{11}
        +\partial_1T_{10}
    )
    \\
    &= \frac{1}{4} [
        (\partial_0T_{00} + \partial_1T_{10})
        - i (\partial_0T_{01} + \partial_1T_{11})
    ]
    = 0
\end{aligned}
$$

Similarly, we can show that $\partial_zT_{\bar{z} \bar{z}}=0$.
$\blacksquare$

